EulerProject3.v
@@ -6,7 +6,7 @@ Local Open Scope string_scope.
 Local Open Scope clight_scope.
 
 Module Info.
-  Definition version := "3.9".
+  Definition version := "3.11".
   Definition build_number := "".
   Definition build_tag := "".
   Definition build_branch := "".
@@ -16,7 +16,7 @@ Module Info.
   Definition bitsize := 64.
   Definition big_endian := false.
   Definition source_file := "EulerProject3.c".
-  Definition normalized := false.
+  Definition normalized := true.
 End Info.
 
 Definition ___builtin_annot : ident := $"__builtin_annot".
@@ -86,102 +86,110 @@ Definition _t'2 : ident := 129%positive.
 Definition _t'3 : ident := 130%positive.
 Definition _t'4 : ident := 131%positive.
 Definition _t'5 : ident := 132%positive.
+Definition _t'6 : ident := 133%positive.
 
 Definition v_highest := {|
-  gvar_info := tlong;
+  gvar_info := tulong;
   gvar_init := (Init_space 8 :: nil);
   gvar_readonly := false;
   gvar_volatile := false
 |}.
 
 Definition f_factorize := {|
-  fn_return := tlong;
+  fn_return := tulong;
   fn_callconv := cc_default;
-  fn_params := ((_n, tlong) :: (_f, tlong) :: nil);
+  fn_params := ((_n, tulong) :: (_f, tulong) :: nil);
   fn_vars := nil;
-  fn_temps := nil;
+  fn_temps := ((_t'1, tulong) :: nil);
   fn_body :=
 (Ssequence
-  (Sifthenelse (Ebinop Olt (Etempvar _n tlong) (Etempvar _f tlong) tint)
-    (Sreturn (Some (Etempvar _n tlong)))
+  (Sifthenelse (Ebinop Olt (Etempvar _n tulong) (Etempvar _f tulong) tint)
+    (Sreturn (Some (Etempvar _n tulong)))
     Sskip)
   (Ssequence
     (Swhile
-      (Ebinop Oeq (Ebinop Omod (Etempvar _n tlong) (Etempvar _f tlong) tlong)
+      (Ebinop Oeq
+        (Ebinop Omod (Etempvar _n tulong) (Etempvar _f tulong) tulong)
         (Econst_int (Int.repr 0) tint) tint)
       (Ssequence
-        (Sset _n (Ebinop Odiv (Etempvar _n tlong) (Etempvar _f tlong) tlong))
-        (Sifthenelse (Ebinop Ogt (Etempvar _f tlong) (Evar _highest tlong)
-                       tint)
-          (Sassign (Evar _highest tlong) (Etempvar _f tlong))
-          Sskip)))
-    (Sreturn (Some (Etempvar _n tlong)))))
+        (Sset _n
+          (Ebinop Odiv (Etempvar _n tulong) (Etempvar _f tulong) tulong))
+        (Ssequence
+          (Sset _t'1 (Evar _highest tulong))
+          (Sifthenelse (Ebinop Ogt (Etempvar _f tulong)
+                         (Etempvar _t'1 tulong) tint)
+            (Sassign (Evar _highest tulong) (Etempvar _f tulong))
+            Sskip))))
+    (Sreturn (Some (Etempvar _n tulong)))))
 |}.
 
 Definition f_find := {|
-  fn_return := tlong;
+  fn_return := tulong;
   fn_callconv := cc_default;
-  fn_params := ((_n, tlong) :: nil);
+  fn_params := ((_n, tulong) :: nil);
   fn_vars := nil;
-  fn_temps := ((_i, tlong) :: (_t'5, tlong) :: (_t'4, tlong) ::
-               (_t'3, tlong) :: (_t'2, tlong) :: (_t'1, tlong) :: nil);
+  fn_temps := ((_i, tulong) :: (_t'5, tulong) :: (_t'4, tulong) ::
+               (_t'3, tulong) :: (_t'2, tulong) :: (_t'1, tulong) ::
+               (_t'6, tulong) :: nil);
   fn_body :=
 (Ssequence
-  (Sassign (Evar _highest tlong) (Econst_int (Int.repr 1) tint))
+  (Sassign (Evar _highest tulong) (Econst_int (Int.repr 1) tint))
   (Ssequence
     (Ssequence
       (Scall (Some _t'1)
-        (Evar _factorize (Tfunction (Tcons tlong (Tcons tlong Tnil)) tlong
+        (Evar _factorize (Tfunction (Tcons tulong (Tcons tulong Tnil)) tulong
                            cc_default))
-        ((Etempvar _n tlong) :: (Econst_int (Int.repr 2) tint) :: nil))
-      (Sset _n (Etempvar _t'1 tlong)))
+        ((Etempvar _n tulong) :: (Econst_int (Int.repr 2) tint) :: nil))
+      (Sset _n (Etempvar _t'1 tulong)))
     (Ssequence
       (Ssequence
         (Scall (Some _t'2)
-          (Evar _factorize (Tfunction (Tcons tlong (Tcons tlong Tnil)) tlong
-                             cc_default))
-          ((Etempvar _n tlong) :: (Econst_int (Int.repr 3) tint) :: nil))
-        (Sset _n (Etempvar _t'2 tlong)))
+          (Evar _factorize (Tfunction (Tcons tulong (Tcons tulong Tnil))
+                             tulong cc_default))
+          ((Etempvar _n tulong) :: (Econst_int (Int.repr 3) tint) :: nil))
+        (Sset _n (Etempvar _t'2 tulong)))
       (Ssequence
-        (Sifthenelse (Ebinop Oge (Etempvar _n tlong)
+        (Sifthenelse (Ebinop Oge (Etempvar _n tulong)
                        (Econst_int (Int.repr 5) tint) tint)
           (Ssequence
-            (Sset _i (Ecast (Econst_int (Int.repr 5) tint) tlong))
+            (Sset _i (Ecast (Econst_int (Int.repr 5) tint) tulong))
             (Sloop
               (Ssequence
                 (Sifthenelse (Ebinop Ole
-                               (Ebinop Omul (Etempvar _i tlong)
-                                 (Etempvar _i tlong) tlong)
-                               (Etempvar _n tlong) tint)
+                               (Ebinop Omul (Etempvar _i tulong)
+                                 (Etempvar _i tulong) tulong)
+                               (Etempvar _n tulong) tint)
                   Sskip
                   Sbreak)
                 (Ssequence
                   (Ssequence
                     (Scall (Some _t'3)
                       (Evar _factorize (Tfunction
-                                         (Tcons tlong (Tcons tlong Tnil))
-                                         tlong cc_default))
-                      ((Etempvar _n tlong) :: (Etempvar _i tlong) :: nil))
-                    (Sset _n (Etempvar _t'3 tlong)))
+                                         (Tcons tulong (Tcons tulong Tnil))
+                                         tulong cc_default))
+                      ((Etempvar _n tulong) :: (Etempvar _i tulong) :: nil))
+                    (Sset _n (Etempvar _t'3 tulong)))
                   (Ssequence
                     (Scall (Some _t'4)
                       (Evar _factorize (Tfunction
-                                         (Tcons tlong (Tcons tlong Tnil))
-                                         tlong cc_default))
-                      ((Etempvar _n tlong) ::
-                       (Ebinop Oadd (Etempvar _i tlong)
-                         (Econst_int (Int.repr 2) tint) tlong) :: nil))
-                    (Sset _n (Etempvar _t'4 tlong)))))
+                                         (Tcons tulong (Tcons tulong Tnil))
+                                         tulong cc_default))
+                      ((Etempvar _n tulong) ::
+                       (Ebinop Oadd (Etempvar _i tulong)
+                         (Econst_int (Int.repr 2) tint) tulong) :: nil))
+                    (Sset _n (Etempvar _t'4 tulong)))))
               (Sset _i
-                (Ebinop Oadd (Etempvar _i tlong)
-                  (Econst_int (Int.repr 6) tint) tlong))))
+                (Ebinop Oadd (Etempvar _i tulong)
+                  (Econst_int (Int.repr 6) tint) tulong))))
           Sskip)
         (Ssequence
-          (Sifthenelse (Ebinop Oeq (Etempvar _n tlong)
+          (Sifthenelse (Ebinop Oeq (Etempvar _n tulong)
                          (Econst_int (Int.repr 1) tint) tint)
-            (Sset _t'5 (Ecast (Evar _highest tlong) tlong))
-            (Sset _t'5 (Ecast (Etempvar _n tlong) tlong)))
-          (Sreturn (Some (Etempvar _t'5 tlong))))))))
+            (Ssequence
+              (Sset _t'6 (Evar _highest tulong))
+              (Sset _t'5 (Ecast (Etempvar _t'6 tulong) tulong)))
+            (Sset _t'5 (Ecast (Etempvar _n tulong) tulong)))
+          (Sreturn (Some (Etempvar _t'5 tulong))))))))
 |}.
 
 Definition f_main := {|
@@ -189,14 +197,14 @@ Definition f_main := {|
   fn_callconv := cc_default;
   fn_params := nil;
   fn_vars := nil;
-  fn_temps := ((_t'1, tlong) :: nil);
+  fn_temps := ((_t'1, tulong) :: nil);
   fn_body :=
 (Ssequence
   (Ssequence
     (Scall (Some _t'1)
-      (Evar _find (Tfunction (Tcons tlong Tnil) tlong cc_default))
+      (Evar _find (Tfunction (Tcons tulong Tnil) tulong cc_default))
       ((Econst_long (Int64.repr 600851475143) tlong) :: nil))
-    (Sreturn (Some (Etempvar _t'1 tlong))))
+    (Sreturn (Some (Etempvar _t'1 tulong))))
   (Sreturn (Some (Econst_int (Int.repr 0) tint))))
 |}.
 
@@ -204,7 +212,93 @@ Definition composites : list composite_definition :=
 nil.
 
 Definition global_definitions : list (ident * globdef fundef type) :=
-((___builtin_bswap64,
+((___compcert_va_int32,
+   Gfun(External (EF_runtime "__compcert_va_int32"
+                   (mksignature (AST.Tlong :: nil) AST.Tint cc_default))
+     (Tcons (tptr tvoid) Tnil) tuint cc_default)) ::
+ (___compcert_va_int64,
+   Gfun(External (EF_runtime "__compcert_va_int64"
+                   (mksignature (AST.Tlong :: nil) AST.Tlong cc_default))
+     (Tcons (tptr tvoid) Tnil) tulong cc_default)) ::
+ (___compcert_va_float64,
+   Gfun(External (EF_runtime "__compcert_va_float64"
+                   (mksignature (AST.Tlong :: nil) AST.Tfloat cc_default))
+     (Tcons (tptr tvoid) Tnil) tdouble cc_default)) ::
+ (___compcert_va_composite,
+   Gfun(External (EF_runtime "__compcert_va_composite"
+                   (mksignature (AST.Tlong :: AST.Tlong :: nil) AST.Tlong
+                     cc_default)) (Tcons (tptr tvoid) (Tcons tulong Tnil))
+     (tptr tvoid) cc_default)) ::
+ (___compcert_i64_dtos,
+   Gfun(External (EF_runtime "__compcert_i64_dtos"
+                   (mksignature (AST.Tfloat :: nil) AST.Tlong cc_default))
+     (Tcons tdouble Tnil) tlong cc_default)) ::
+ (___compcert_i64_dtou,
+   Gfun(External (EF_runtime "__compcert_i64_dtou"
+                   (mksignature (AST.Tfloat :: nil) AST.Tlong cc_default))
+     (Tcons tdouble Tnil) tulong cc_default)) ::
+ (___compcert_i64_stod,
+   Gfun(External (EF_runtime "__compcert_i64_stod"
+                   (mksignature (AST.Tlong :: nil) AST.Tfloat cc_default))
+     (Tcons tlong Tnil) tdouble cc_default)) ::
+ (___compcert_i64_utod,
+   Gfun(External (EF_runtime "__compcert_i64_utod"
+                   (mksignature (AST.Tlong :: nil) AST.Tfloat cc_default))
+     (Tcons tulong Tnil) tdouble cc_default)) ::
+ (___compcert_i64_stof,
+   Gfun(External (EF_runtime "__compcert_i64_stof"
+                   (mksignature (AST.Tlong :: nil) AST.Tsingle cc_default))
+     (Tcons tlong Tnil) tfloat cc_default)) ::
+ (___compcert_i64_utof,
+   Gfun(External (EF_runtime "__compcert_i64_utof"
+                   (mksignature (AST.Tlong :: nil) AST.Tsingle cc_default))
+     (Tcons tulong Tnil) tfloat cc_default)) ::
+ (___compcert_i64_sdiv,
+   Gfun(External (EF_runtime "__compcert_i64_sdiv"
+                   (mksignature (AST.Tlong :: AST.Tlong :: nil) AST.Tlong
+                     cc_default)) (Tcons tlong (Tcons tlong Tnil)) tlong
+     cc_default)) ::
+ (___compcert_i64_udiv,
+   Gfun(External (EF_runtime "__compcert_i64_udiv"
+                   (mksignature (AST.Tlong :: AST.Tlong :: nil) AST.Tlong
+                     cc_default)) (Tcons tulong (Tcons tulong Tnil)) tulong
+     cc_default)) ::
+ (___compcert_i64_smod,
+   Gfun(External (EF_runtime "__compcert_i64_smod"
+                   (mksignature (AST.Tlong :: AST.Tlong :: nil) AST.Tlong
+                     cc_default)) (Tcons tlong (Tcons tlong Tnil)) tlong
+     cc_default)) ::
+ (___compcert_i64_umod,
+   Gfun(External (EF_runtime "__compcert_i64_umod"
+                   (mksignature (AST.Tlong :: AST.Tlong :: nil) AST.Tlong
+                     cc_default)) (Tcons tulong (Tcons tulong Tnil)) tulong
+     cc_default)) ::
+ (___compcert_i64_shl,
+   Gfun(External (EF_runtime "__compcert_i64_shl"
+                   (mksignature (AST.Tlong :: AST.Tint :: nil) AST.Tlong
+                     cc_default)) (Tcons tlong (Tcons tint Tnil)) tlong
+     cc_default)) ::
+ (___compcert_i64_shr,
+   Gfun(External (EF_runtime "__compcert_i64_shr"
+                   (mksignature (AST.Tlong :: AST.Tint :: nil) AST.Tlong
+                     cc_default)) (Tcons tulong (Tcons tint Tnil)) tulong
+     cc_default)) ::
+ (___compcert_i64_sar,
+   Gfun(External (EF_runtime "__compcert_i64_sar"
+                   (mksignature (AST.Tlong :: AST.Tint :: nil) AST.Tlong
+                     cc_default)) (Tcons tlong (Tcons tint Tnil)) tlong
+     cc_default)) ::
+ (___compcert_i64_smulh,
+   Gfun(External (EF_runtime "__compcert_i64_smulh"
+                   (mksignature (AST.Tlong :: AST.Tlong :: nil) AST.Tlong
+                     cc_default)) (Tcons tlong (Tcons tlong Tnil)) tlong
+     cc_default)) ::
+ (___compcert_i64_umulh,
+   Gfun(External (EF_runtime "__compcert_i64_umulh"
+                   (mksignature (AST.Tlong :: AST.Tlong :: nil) AST.Tlong
+                     cc_default)) (Tcons tulong (Tcons tulong Tnil)) tulong
+     cc_default)) ::
+ (___builtin_bswap64,
    Gfun(External (EF_builtin "__builtin_bswap64"
                    (mksignature (AST.Tlong :: nil) AST.Tlong cc_default))
      (Tcons tulong Tnil) tulong cc_default)) ::
@@ -307,23 +401,6 @@ Definition global_definitions : list (ident * globdef fundef type) :=
    Gfun(External (EF_builtin "__builtin_va_end"
                    (mksignature (AST.Tlong :: nil) AST.Tvoid cc_default))
      (Tcons (tptr tvoid) Tnil) tvoid cc_default)) ::
- (___compcert_va_int32,
-   Gfun(External (EF_external "__compcert_va_int32"
-                   (mksignature (AST.Tlong :: nil) AST.Tint cc_default))
-     (Tcons (tptr tvoid) Tnil) tuint cc_default)) ::
- (___compcert_va_int64,
-   Gfun(External (EF_external "__compcert_va_int64"
-                   (mksignature (AST.Tlong :: nil) AST.Tlong cc_default))
-     (Tcons (tptr tvoid) Tnil) tulong cc_default)) ::
- (___compcert_va_float64,
-   Gfun(External (EF_external "__compcert_va_float64"
-                   (mksignature (AST.Tlong :: nil) AST.Tfloat cc_default))
-     (Tcons (tptr tvoid) Tnil) tdouble cc_default)) ::
- (___compcert_va_composite,
-   Gfun(External (EF_external "__compcert_va_composite"
-                   (mksignature (AST.Tlong :: AST.Tlong :: nil) AST.Tlong
-                     cc_default)) (Tcons (tptr tvoid) (Tcons tulong Tnil))
-     (tptr tvoid) cc_default)) ::
  (___builtin_unreachable,
    Gfun(External (EF_builtin "__builtin_unreachable"
                    (mksignature nil AST.Tvoid cc_default)) Tnil tvoid
@@ -332,75 +409,6 @@ Definition global_definitions : list (ident * globdef fundef type) :=
    Gfun(External (EF_builtin "__builtin_expect"
                    (mksignature (AST.Tlong :: AST.Tlong :: nil) AST.Tlong
                      cc_default)) (Tcons tlong (Tcons tlong Tnil)) tlong
-     cc_default)) ::
- (___compcert_i64_dtos,
-   Gfun(External (EF_runtime "__compcert_i64_dtos"
-                   (mksignature (AST.Tfloat :: nil) AST.Tlong cc_default))
-     (Tcons tdouble Tnil) tlong cc_default)) ::
- (___compcert_i64_dtou,
-   Gfun(External (EF_runtime "__compcert_i64_dtou"
-                   (mksignature (AST.Tfloat :: nil) AST.Tlong cc_default))
-     (Tcons tdouble Tnil) tulong cc_default)) ::
- (___compcert_i64_stod,
-   Gfun(External (EF_runtime "__compcert_i64_stod"
-                   (mksignature (AST.Tlong :: nil) AST.Tfloat cc_default))
-     (Tcons tlong Tnil) tdouble cc_default)) ::
- (___compcert_i64_utod,
-   Gfun(External (EF_runtime "__compcert_i64_utod"
-                   (mksignature (AST.Tlong :: nil) AST.Tfloat cc_default))
-     (Tcons tulong Tnil) tdouble cc_default)) ::
- (___compcert_i64_stof,
-   Gfun(External (EF_runtime "__compcert_i64_stof"
-                   (mksignature (AST.Tlong :: nil) AST.Tsingle cc_default))
-     (Tcons tlong Tnil) tfloat cc_default)) ::
- (___compcert_i64_utof,
-   Gfun(External (EF_runtime "__compcert_i64_utof"
-                   (mksignature (AST.Tlong :: nil) AST.Tsingle cc_default))
-     (Tcons tulong Tnil) tfloat cc_default)) ::
- (___compcert_i64_sdiv,
-   Gfun(External (EF_runtime "__compcert_i64_sdiv"
-                   (mksignature (AST.Tlong :: AST.Tlong :: nil) AST.Tlong
-                     cc_default)) (Tcons tlong (Tcons tlong Tnil)) tlong
-     cc_default)) ::
- (___compcert_i64_udiv,
-   Gfun(External (EF_runtime "__compcert_i64_udiv"
-                   (mksignature (AST.Tlong :: AST.Tlong :: nil) AST.Tlong
-                     cc_default)) (Tcons tulong (Tcons tulong Tnil)) tulong
-     cc_default)) ::
- (___compcert_i64_smod,
-   Gfun(External (EF_runtime "__compcert_i64_smod"
-                   (mksignature (AST.Tlong :: AST.Tlong :: nil) AST.Tlong
-                     cc_default)) (Tcons tlong (Tcons tlong Tnil)) tlong
-     cc_default)) ::
- (___compcert_i64_umod,
-   Gfun(External (EF_runtime "__compcert_i64_umod"
-                   (mksignature (AST.Tlong :: AST.Tlong :: nil) AST.Tlong
-                     cc_default)) (Tcons tulong (Tcons tulong Tnil)) tulong
-     cc_default)) ::
- (___compcert_i64_shl,
-   Gfun(External (EF_runtime "__compcert_i64_shl"
-                   (mksignature (AST.Tlong :: AST.Tint :: nil) AST.Tlong
-                     cc_default)) (Tcons tlong (Tcons tint Tnil)) tlong
-     cc_default)) ::
- (___compcert_i64_shr,
-   Gfun(External (EF_runtime "__compcert_i64_shr"
-                   (mksignature (AST.Tlong :: AST.Tint :: nil) AST.Tlong
-                     cc_default)) (Tcons tulong (Tcons tint Tnil)) tulong
-     cc_default)) ::
- (___compcert_i64_sar,
-   Gfun(External (EF_runtime "__compcert_i64_sar"
-                   (mksignature (AST.Tlong :: AST.Tint :: nil) AST.Tlong
-                     cc_default)) (Tcons tlong (Tcons tint Tnil)) tlong
-     cc_default)) ::
- (___compcert_i64_smulh,
-   Gfun(External (EF_runtime "__compcert_i64_smulh"
-                   (mksignature (AST.Tlong :: AST.Tlong :: nil) AST.Tlong
-                     cc_default)) (Tcons tlong (Tcons tlong Tnil)) tlong
-     cc_default)) ::
- (___compcert_i64_umulh,
-   Gfun(External (EF_runtime "__compcert_i64_umulh"
-                   (mksignature (AST.Tlong :: AST.Tlong :: nil) AST.Tlong
-                     cc_default)) (Tcons tulong (Tcons tulong Tnil)) tulong
      cc_default)) ::
  (___builtin_fmax,
    Gfun(External (EF_builtin "__builtin_fmax"
@@ -474,21 +482,21 @@ Definition public_idents : list ident :=
  ___builtin_read32_reversed :: ___builtin_read16_reversed ::
  ___builtin_fnmsub :: ___builtin_fnmadd :: ___builtin_fmsub ::
  ___builtin_fmadd :: ___builtin_fmin :: ___builtin_fmax ::
+ ___builtin_expect :: ___builtin_unreachable :: ___builtin_va_end ::
+ ___builtin_va_copy :: ___builtin_va_arg :: ___builtin_va_start ::
+ ___builtin_membar :: ___builtin_annot_intval :: ___builtin_annot ::
+ ___builtin_sel :: ___builtin_memcpy_aligned :: ___builtin_sqrt ::
+ ___builtin_fsqrt :: ___builtin_fabsf :: ___builtin_fabs ::
+ ___builtin_ctzll :: ___builtin_ctzl :: ___builtin_ctz :: ___builtin_clzll ::
+ ___builtin_clzl :: ___builtin_clz :: ___builtin_bswap16 ::
+ ___builtin_bswap32 :: ___builtin_bswap :: ___builtin_bswap64 ::
  ___compcert_i64_umulh :: ___compcert_i64_smulh :: ___compcert_i64_sar ::
  ___compcert_i64_shr :: ___compcert_i64_shl :: ___compcert_i64_umod ::
  ___compcert_i64_smod :: ___compcert_i64_udiv :: ___compcert_i64_sdiv ::
  ___compcert_i64_utof :: ___compcert_i64_stof :: ___compcert_i64_utod ::
  ___compcert_i64_stod :: ___compcert_i64_dtou :: ___compcert_i64_dtos ::
- ___builtin_expect :: ___builtin_unreachable :: ___compcert_va_composite ::
- ___compcert_va_float64 :: ___compcert_va_int64 :: ___compcert_va_int32 ::
- ___builtin_va_end :: ___builtin_va_copy :: ___builtin_va_arg ::
- ___builtin_va_start :: ___builtin_membar :: ___builtin_annot_intval ::
- ___builtin_annot :: ___builtin_sel :: ___builtin_memcpy_aligned ::
- ___builtin_sqrt :: ___builtin_fsqrt :: ___builtin_fabsf ::
- ___builtin_fabs :: ___builtin_ctzll :: ___builtin_ctzl :: ___builtin_ctz ::
- ___builtin_clzll :: ___builtin_clzl :: ___builtin_clz ::
- ___builtin_bswap16 :: ___builtin_bswap32 :: ___builtin_bswap ::
- ___builtin_bswap64 :: nil).
+ ___compcert_va_composite :: ___compcert_va_float64 ::
+ ___compcert_va_int64 :: ___compcert_va_int32 :: nil).
 
 Definition prog : Clight.program := 
   mkprogram composites global_definitions public_idents _main Logic.I.
